wip

code/experimental/Hacl.Impl.LowLevel.fst
@@ -74,6 +74,70 @@ let add6_0 x y result =
   
   cc2
 
+
+inline_for_extraction noextract
+val add6_with_carry0: cc2: uint64 ->  x: felem6_buffer -> y: felem6_buffer-> result: felem6_buffer -> Stack uint64 
+  (requires fun h -> live h x /\ live h y /\ live h result /\ eq_or_disjoint x result /\ eq_or_disjoint y result /\ uint_v cc2 <= 1)
+  (ensures fun h0 c h1 -> modifies (loc result) h0 h1 /\ 
+    v c <= 1 /\
+    (
+      let r0 = Lib.Sequence.index (as_seq h1 result) 0 in 
+      let r1 = Lib.Sequence.index (as_seq h1 result) 1 in 
+      let r2 = Lib.Sequence.index (as_seq h1 result) 2 in 
+  
+      let a0 = Lib.Sequence.index (as_seq h0 x) 0 in 
+      let a1 = Lib.Sequence.index (as_seq h0 x) 1 in 
+      let a2 = Lib.Sequence.index (as_seq h0 x) 2 in 
+
+      let b0 = Lib.Sequence.index (as_seq h0 y) 0 in 
+      let b1 = Lib.Sequence.index (as_seq h0 y) 1 in 
+      let b2 = Lib.Sequence.index (as_seq h0 y) 2 in 
+
+      let r3_0 = Lib.Sequence.index (as_seq h0 result) 3 in 
+      let r3_1 = Lib.Sequence.index (as_seq h1 result) 3 in 
+      
+      let r4_0 = Lib.Sequence.index (as_seq h0 result) 4 in 
+      let r4_1 = Lib.Sequence.index (as_seq h1 result) 4 in 
+      
+      let r5_0 = Lib.Sequence.index (as_seq h0 result) 5 in 
+      let r5_1 = Lib.Sequence.index (as_seq h1 result) 5 in 
+
+      v r0 + v r1 * pow2 (1 * 64) + v r2 * pow2 (2 * 64) + v c * pow2 (3 * 64) ==
+      v a0 + v b0 + v a1 * pow2 64 + v b1 * pow2 64 + v a2 * pow2 (2 * 64) + v b2 * pow2 (2 * 64) + uint_v cc2 /\
+
+      r3_0 == r3_1 /\ r4_0 == r4_1 /\ r5_0 == r5_1
+
+    )
+  )
+
+
+let add6_with_carry0 cc2 x y result =
+  let h0 = ST.get() in 
+  assert_norm (pow2 64 * pow2 64 = pow2 (2 * 64));
+  assert_norm (pow2 64 * pow2 64 * pow2 64 = pow2 (3 * 64));
+  let r0 = sub result (size 0) (size 1) in 
+  let r1 = sub result (size 1) (size 1) in 
+  let r2 = sub result (size 2) (size 1) in 
+
+  let r3 = sub result (size 3) (size 1) in 
+  let r4 = sub result (size 4) (size 1) in 
+  let r5 = sub result (size 5) (size 1) in 
+
+  assert(Lib.Sequence.index (as_seq h0 r3) 0 == Lib.Sequence.index (as_seq h0 result) 3);
+  assert(Lib.Sequence.index (as_seq h0 r4) 0 == Lib.Sequence.index (as_seq h0 result) 4);
+  assert(Lib.Sequence.index (as_seq h0 r5) 0 == Lib.Sequence.index (as_seq h0 result) 5);
+
+  assert(let r4_0 = as_seq h0 r1 in let r0_ = as_seq h0 result in Seq.index r0_ 1 == Seq.index r4_0 0);
+  assert(let r5_0 = as_seq h0 r2 in let r0_ = as_seq h0 result in Seq.index r0_ 2 == Seq.index r5_0 0);
+
+  let cc0 = add_carry_u64 cc2 x.(0ul) y.(0ul) r0 in 
+  let cc1 = add_carry_u64 cc0 x.(1ul) y.(1ul) r1 in 
+  let cc2 = add_carry_u64 cc1 x.(2ul) y.(2ul) r2 in 
+  
+  cc2
+
+
+
 inline_for_extraction noextract
 val add6_1: x: felem6_buffer -> y: felem6_buffer -> result: felem6_buffer -> cc2: uint64 -> 
   Stack uint64 
@@ -152,7 +216,308 @@ val add6: x: felem6_buffer -> y: felem6_buffer -> result: felem6_buffer ->
     (ensures fun h0 c h1 -> modifies (loc result) h0 h1 /\ v c <= 1 /\ 
       as_nat6 h1 result + v c * pow2 (6 * 64) == as_nat6 h0 x + as_nat6 h0 y)   
 
-
 let add6 x y result =    
   let cc2 = add6_0 x y result in 
   add6_1 x y result cc2
+
+
+val add6_with_carry: c: uint64 -> x: felem6_buffer -> y: felem6_buffer -> result: felem6_buffer -> 
+  Stack uint64 
+    (requires fun h -> uint_v c <= 1 /\ live h x /\ live h y /\ live h result /\ 
+      eq_or_disjoint x result /\ eq_or_disjoint y result)
+    (ensures fun h0 cc5 h1 -> modifies (loc result) h0 h1 /\ uint_v cc5 <= 1 /\
+      as_nat6 h1 result + v cc5 * pow2 (6 * 64) == as_nat6 h0 x + as_nat6 h0 y + v c)
+
+let add6_with_carry c x y result = 
+  let cc2 = add6_with_carry0 c x y result in 
+  let cc5 = add6_1 x y result cc2 in 
+  cc5
+  
+
+val lemmaFelem6asFelem12: x: felem12_buffer -> h: mem -> Lemma
+    (
+      let x0 = gsub x (size 0) (size 6) in 
+      let x1 = gsub x (size 6) (size 6) in 
+      as_nat6 h x0 + as_nat6 h x1 * pow2 (6 * 64) == as_nat12 h x
+    )
+
+let lemmaFelem6asFelem12 x h = 
+     assert_norm (pow2 (1 * 64) * pow2 (6 * 64) = pow2 (7 * 64));
+    assert_norm (pow2 (2 * 64) * pow2 (6 * 64) = pow2 (8 * 64));
+    assert_norm (pow2 (3 * 64) * pow2 (6 * 64) = pow2 (9 * 64));
+    assert_norm (pow2 (4 * 64) * pow2 (6 * 64) = pow2 (10 * 64));
+    assert_norm (pow2 (5 * 64) * pow2 (6 * 64) = pow2 (11 * 64));
+    assert_norm (pow2 (6 * 64) * pow2 (6 * 64) = pow2 (12 * 64))
+
+
+val add12: x: felem12_buffer -> y: felem12_buffer -> result: felem12_buffer -> Stack uint64
+  (requires fun h -> live h x /\ live h y /\ live h result /\ eq_or_disjoint x result /\ eq_or_disjoint y result)
+  (ensures (fun h0 c h1 -> modifies (loc result) h0 h1 /\ v c <= 1 /\
+    as_nat12 h1 result + v c * pow2 (12 * 64) == as_nat12 h0 x + as_nat12 h0 y))
+
+let add12 x y result = 
+  let open FStar.Tactics in 
+  let open FStar.Tactics.Canon in 
+  assert_norm (pow2 (6 * 64) * pow2 (6 * 64) = pow2 (12 * 64));
+
+  let h0 = ST.get() in 
+
+    let a0 = sub x (size 0) (size 6) in 
+    let a1 = sub x (size 6) (size 6) in 
+
+
+    let b0 = sub y (size 0) (size 6) in 
+    let b1 = sub y (size 6) (size 6) in 
+
+    let c0 = sub result (size 0) (size 6) in 
+    let c1 = sub result (size 6) (size 6) in 
+
+    let carry0 = add6 a0 b0 c0 in 
+    let carry1 = add6_with_carry carry0 a1 b1 c1 in 
+
+  let h1 = ST.get() in 
+  
+    assert_by_tactic (pow2 (6 * 64) * (as_nat6 h1 c1 + v carry1 * pow2 (6 * 64)) == as_nat6 h1 c1 * pow2 (6 * 64) + v carry1 * pow2 (6 * 64) * pow2 (6 * 64)) canon;
+    assert_by_tactic (pow2 (6 * 64) * (as_nat6 h0 a1 + as_nat6 h0 b1 + v carry0) = as_nat6 h0 a1 * pow2 (6 * 64) + as_nat6 h0 b1 * pow2 (6 * 64) +  v carry0 * pow2 (6 * 64)) canon;
+
+
+    calc (==) {
+      as_nat12 h1 result + v carry1 * pow2 (12 * 64);
+      (==) {lemmaFelem6asFelem12 result h1}
+      as_nat6 h1 c0 + as_nat6 h1 c1 * pow2 (6 * 64) + v carry1 * pow2 (12 * 64);
+      (==) {assert((as_nat6 h1 c1) * pow2 (6 * 64) == (- v carry1 * pow2 (6 * 64)  + as_nat6 h0 a1 + as_nat6 h0 b1 + v carry0) * pow2 (6 * 64))}
+      as_nat6 h1 c0 + (- v carry1 * pow2 (6 * 64)  + as_nat6 h0 a1 + as_nat6 h0 b1 + v carry0) * pow2 (6 * 64) + v carry1 * pow2 (12 * 64);
+      (==) {}
+      (as_nat6 h0 a0 + as_nat6 h0 a1 * pow2 (6 * 64)) + (as_nat6 h0 b0  + as_nat6 h0 b1 * pow2 (6 * 64));
+      (==) {lemmaFelem6asFelem12 x h0}
+      as_nat12 h0 x + (as_nat6 h0 b0  + as_nat6 h0 b1 * pow2 (6 * 64));
+      (==) {lemmaFelem6asFelem12 y h0}
+      as_nat12 h0 x + as_nat12 h0 y;};
+
+    carry1
+
+
+val mul64: x: uint64 -> y: uint64 -> result: lbuffer uint64 (size 1) -> temp: lbuffer uint64 (size 1) ->
+  Stack unit
+    (requires fun h -> live h result /\ live h temp /\ disjoint result temp)
+  (ensures fun h0 _ h1 -> modifies (loc result |+| loc temp) h0 h1 /\ 
+    (
+      let h0 = Seq.index (as_seq h1 temp) 0 in 
+      let result = Seq.index (as_seq h1 result) 0 in 
+      uint_v result + uint_v h0 * pow2 64 = uint_v x * uint_v y     
+      )
+    )
+
+let mul64 x y result temp = 
+  let res = mul64_wide x y in 
+  let l0, h0 = to_u64 res, to_u64 (res >>. 64ul) in 
+  upd result (size 0) l0;
+  upd temp (size 0) h0
+
+
+
+val mult64_0il: x: ilbuffer uint64 (size 6) -> u: uint64 -> result:  lbuffer uint64 (size 1) -> temp: lbuffer uint64 (size 1) -> Stack unit 
+  (requires fun h -> live h x /\ live h result /\ live h temp /\ disjoint result temp)
+  (ensures fun h0 _ h1 -> 
+    let result_ = Seq.index (as_seq h1 result) 0 in 
+    let c = Seq.index (as_seq h1 temp) 0 in 
+    let f0 = Seq.index (as_seq h0 x) 0 in 
+    uint_v result_ + uint_v c * pow2 64 = uint_v f0 * uint_v u /\ modifies (loc result |+| loc temp) h0 h1)
+
+let mult64_0il x u result temp = 
+  let f0 = index x (size 0) in 
+  mul64 f0 u result temp
+
+
+val mult64_c: x: uint64 -> u: uint64 -> cin: uint64{uint_v cin <= 1} -> result: lbuffer uint64 (size 1) -> temp: lbuffer uint64 (size 1) -> Stack uint64 
+  (requires fun h -> live h result /\ live h temp /\ disjoint result temp)
+  (ensures fun h0 c2 h1 -> modifies (loc result |+| loc temp) h0 h1 /\ uint_v c2 <= 1 /\
+    (
+      let r = Seq.index (as_seq h1 result) 0 in 
+      let h1 = Seq.index (as_seq h1 temp) 0 in 
+      let h0 = Seq.index (as_seq h0 temp) 0 in 
+      uint_v r + uint_v c2 * pow2 64 == uint_v x * uint_v u - uint_v h1 * pow2 64 + uint_v h0 + uint_v cin)
+)
+
+let mult64_c x u cin result temp = 
+  let h = index temp (size 0) in 
+  mul64 x u result temp;
+  let l = index result (size 0) in     
+  add_carry_u64 cin l h result
+
+
+val lemma_mult: a: int -> b: int -> c: int -> d: int -> e: int -> f: nat ->  Lemma
+   (requires (a = b + c + d + e))
+   (ensures (a * f = b * f + c * f + d * f + e * f))
+
+let lemma_mult a b c d e f = ()
+
+
+val lemma_mult5: a: int -> b: int -> c: int -> d: int -> e: int -> f: int -> j: nat -> Lemma
+   (requires (a = b + c + d + e + f))
+   (ensures (a * j = b * j + c * j + d * j + e * j + f * j ))
+
+let lemma_mult5 a b c d e f j = ()
+
+
+val mul1_il0: f: ilbuffer uint64 (size 6) -> u: uint64 -> result: lbuffer uint64 (size 6) -> temp: lbuffer uint64 (size 1) -> Stack uint64
+  (requires fun h -> live h result /\ live h f /\ live h temp /\  disjoint result temp)
+  (ensures fun h0 c h1 -> modifies (loc result |+| loc temp) h0 h1  /\
+    uint_v c <= 1 /\
+    
+      uint_v (Seq.index (as_seq h1 result) 0) + 
+      uint_v (Seq.index (as_seq h1 result) 1) * pow2 64 +
+      uint_v (Seq.index (as_seq h1 result) 2) * pow2 (2 * 64) + 
+      uint_v (Seq.index (as_seq h1 result) 3) * pow2 (3 * 64) + 
+      uint_v c * pow2 (4 * 64) + uint_v (Seq.index (as_seq h1 temp) 0) * pow2 (4 * 64) ==
+      
+      uint_v (Seq.index (as_seq h0 f) 0) * uint_v u + 
+      uint_v (Seq.index (as_seq h0 f) 1) * uint_v u * pow2 64 + 
+      uint_v (Seq.index (as_seq h0 f) 2) * uint_v u * pow2 (2 * 64) + 
+      uint_v (Seq.index (as_seq h0 f) 3) * uint_v u * pow2 (3 * 64)
+  )
+
+
+let mul1_il0 f u result temp = 
+  let h0 = ST.get() in 
+
+  let f0 = index f (size 0) in 
+  let f1 = index f (size 1) in 
+  let f2 = index f (size 2) in 
+  let f3 = index f (size 3) in 
+
+  let o0 = sub result (size 0) (size 1) in 
+  let o1 = sub result (size 1) (size 1) in 
+  let o2 = sub result (size 2) (size 1) in 
+  let o3 = sub result (size 3) (size 1) in 
+
+  assert_norm (pow2 64 * pow2 64 = pow2 (2 * 64));
+  assert_norm (pow2 64 * pow2 (2 * 64) = pow2 (3 * 64));
+  assert_norm (pow2 64 * pow2 (3 * 64) = pow2 (4 * 64));
+
+   mult64_0il f u o0 temp;
+    let h1 = ST.get() in 
+    
+  let c1 = mult64_c f1 u (u64 0) o1 temp in 
+    let h2 = ST.get() in 
+     lemma_mult (uint_v f1 * uint_v u) (uint_v (Seq.index (as_seq h2 o1) 0)) (uint_v c1 * pow2 64) (uint_v (Seq.index (as_seq h2 temp) 0) * pow2 64) (- uint_v (Seq.index (as_seq h1 temp) 0)) (pow2 64); 
+    
+  let c2 = mult64_c f2 u c1 o2 temp in 
+    let h3 = ST.get() in 
+    lemma_mult5 (uint_v f2 * uint_v u) (uint_v (Seq.index (as_seq h3 o2) 0)) (uint_v c2 * pow2 64) (uint_v (Seq.index (as_seq h3 temp) 0) * pow2 64) (- uint_v (Seq.index (as_seq h2 temp) 0)) (- uint_v c1) (pow2 (2 * 64));
+
+  let c3 = mult64_c f3 u c2 o3 temp in 
+    let h4 = ST.get() in 
+    lemma_mult5 (uint_v f3 * uint_v u) (uint_v (Seq.index (as_seq h4 o3) 0)) (uint_v c3 * pow2 64) (uint_v (Seq.index (as_seq h4 temp) 0) * pow2 64) (- uint_v (Seq.index (as_seq h3 temp) 0)) (- uint_v c2) (pow2 (3 * 64));
+
+  c3
+  
+
+
+
+val mul1_il: f:  ilbuffer uint64 (size 6) -> u: uint64 -> result: lbuffer uint64 (size 6) -> Stack uint64
+  (requires fun h -> live h result /\ live h f)
+  (ensures fun h0 c h1 -> modifies (loc result) h0 h1 /\ 
+    as_nat6_il h0 f * uint_v u = uint_v c * pow2 (6 * 64) + as_nat6 h1 result /\ 
+    as_nat6_il h0 f * uint_v u < pow2 (7 * 64) /\
+    uint_v c < pow2 64 - 1 
+  )
+
+
+let mul1_il f u result = 
+  push_frame();
+
+  let temp = create (size 1) (u64 0) in 
+
+  let f4 = index f (size 4) in 
+  let f5 = index f (size 5) in 
+    
+
+  let o4 = sub result (size 4) (size 1) in 
+  let o5 = sub result (size 5) (size 1) in 
+  
+  let c3 = mul1_il0 f u result temp in 
+  let h4 = ST.get() in
+
+  let c4 = mult64_c f4 u c3 o4 temp in 
+    let h5 = ST.get() in 
+    assert(uint_v (Seq.index (as_seq h5 o4) 0) + uint_v c4 * pow2 64 + uint_v (Seq.index (as_seq h5 temp) 0) * pow2 64 - uint_v (Seq.index (as_seq h4 temp) 0) - uint_v c3 == uint_v f4 * uint_v u);
+
+    lemma_mult5 (uint_v f4 * uint_v u) (uint_v (Seq.index (as_seq h5 o4) 0)) (uint_v c4 * pow2 64) (uint_v (Seq.index (as_seq h5 temp) 0) * pow2 64) (- uint_v (Seq.index (as_seq h4 temp) 0)) (- uint_v c3) (pow2 (4 * 64));
+
+     assert(uint_v (Seq.index (as_seq h5 o4) 0) * pow2 (4 * 64) + uint_v c4 * pow2 64 * pow2 (4 * 64) + uint_v (Seq.index (as_seq h5 temp) 0) * pow2 64 * pow2 (4 * 64) - uint_v (Seq.index (as_seq h4 temp) 0) * pow2 (4 * 64) - uint_v c3 * pow2 (4 * 64) == uint_v f4 * uint_v u * pow2 (4 * 64));
+
+
+  let c5 = mult64_c f5 u c4 o5 temp in 
+      let h6 = ST.get() in 
+     assert(uint_v (Seq.index (as_seq h6 o5) 0) + uint_v c5 * pow2 64 + uint_v (Seq.index (as_seq h6 temp) 0) * pow2 64 - uint_v (Seq.index (as_seq h5 temp) 0) - uint_v c4 == uint_v f5 * uint_v u);
+
+    lemma_mult5 (uint_v f5 * uint_v u) (uint_v (Seq.index (as_seq h6 o5) 0)) (uint_v c5 * pow2 64) (uint_v (Seq.index (as_seq h6 temp) 0) * pow2 64) (- uint_v (Seq.index (as_seq h5 temp) 0)) (- uint_v c4) (pow2 (5 * 64));
+
+     assert(uint_v (Seq.index (as_seq h6 o5) 0) * pow2 (5 * 64) + uint_v c5 * pow2 64 * pow2 (5 * 64) + uint_v (Seq.index (as_seq h6 temp) 0) * pow2 64 * pow2 (5 * 64) - uint_v (Seq.index (as_seq h5 temp) 0) * pow2 (5 * 64) - uint_v c4 * pow2 (5 * 64) == uint_v f5 * uint_v u * pow2 (5 * 64));
+
+
+  let temp0 = index temp (size 0) in 
+
+
+  pop_frame();  
+  admit();
+  c5 +! temp0
+
+
+val shortened_mul: a: ilbuffer uint64 (size 6) -> b: uint64 -> result: felem12_buffer -> Stack unit
+  (requires fun h -> live h a /\ live h result)
+  (ensures fun h0 _ h1 -> modifies (loc result) h0 h1 /\ 
+    as_nat6_il h0 a * uint_v b = as_nat12 h1 result)
+
+
+let shortened_mul a b result = 
+  let result0 = sub result (size 0) (size 4) in 
+  let result4 = sub result (size 4) (size 4) in 
+  let c = mul1_il a b result0 in 
+  upd result (size 6) c;
+  upd result (size 7) (u64 0);
+  upd result (size 8) (u64 0);
+  upd result (size 9) (u64 0);
+  upd result (size 10) (u64 0);
+  upd result (size 11) (u64 0)
+  
+
+
+
+inline_for_extraction noextract
+val mod64: a: felem12_buffer -> Stack uint64 
+  (requires fun h -> live h a) 
+  (ensures fun h0 r h1 -> modifies0 h0 h1 /\  as_nat12 h1 a % pow2 64 = uint_v r)
+
+let mod64 a = index a (size 0)
+
+
+val shift12: t: felem12_buffer -> t1: felem12_buffer -> Stack unit 
+  (requires fun h -> live h t /\ live h t1 /\ eq_or_disjoint t t1)
+  (ensures fun h0 _ h1 -> modifies (loc t1) h0 h1 /\ as_nat12 h0 t / pow2 64 = as_nat12 h1 t1)
+
+let shift12 t out = 
+  let t1 = index t (size 1) in 
+  let t2 = index t (size 2) in 
+  let t3 = index t (size 3) in 
+  let t4 = index t (size 4) in 
+  let t5 = index t (size 5) in 
+  let t6 = index t (size 6) in 
+  let t7 = index t (size 7) in 
+  let t8 = index t (size 8) in 
+  let t9 = index t (size 9) in 
+  let t10 = index t (size 10) in 
+  let t11 = index t (size 11) in 
+
+  upd out (size 0) t1;
+  upd out (size 1) t2;
+  upd out (size 2) t3;
+  upd out (size 3) t4;
+  upd out (size 4) t5;
+  upd out (size 5) t6;
+  upd out (size 6) t7;
+  upd out (size 7) t8;  upd out (size 8) t9;
+  upd out (size 9) t10;
+  upd out (size 10) t11;
+  upd out (size 11) (u64 0)
