code/experimental/Hacl.Impl.P384.MontgomeryMultiplication.fst
@@ -7,6 +7,41 @@ module ST = FStar.HyperStack.ST
 open FStar.Math.Lemmas
 open FStar.Mul
 
-(*
-inline_for_extraction noextract
+open Lib.IntTypes
+open Lib.Buffer
 
+open Hacl.Spec.P384.Definition
+open Hacl.Impl.P384.LowLevel
+
+open Hacl.Impl.LowLevel
+
+
+val add12_without_carry1: t: felem12_buffer -> t1: felem12_buffer -> result: felem12_buffer -> Stack unit
+  (requires (fun h -> True))
+  (ensures (fun h0 _ h1 -> as_nat12 h1 result = as_nat12 h0 t + as_nat12 h0 t1))
+
+
+let add12_without_carry1 t t1 result = 
+  let t0 = add12 t t1 result in ()
+
+
+
+val montgomeryMultiplicationRound: t: felem12_buffer -> round: felem12_buffer -> tempBuffer: lbuffer uint64 (size 24) -> 
+  Stack unit
+  (requires fun h -> live h t /\ live h round /\ as_nat12 h t < prime384 * prime384)
+  (ensures fun h0 _ h1 -> modifies (loc round) h0 h1 /\
+    as_nat12 h1 round = (as_nat12 h0 t + prime384 * (as_nat12 h0 t % pow2 64)) / pow2 64
+  )
+
+
+let montgomeryMultiplicationRound t round tempBuffer = 
+  let t2 = sub tempBuffer (size 0) (size 12) in 
+  let t3 = sub tempBuffer (size 12) (size 12) in 
+ 
+  let t1 = mod64 t in 
+  
+    recall_contents prime384_buffer (Lib.Sequence.of_list p384_prime_list);
+  shortened_mul prime384_buffer t1 t2;
+  add12_without_carry1 t t2 t3;
+  shift12 t3 round
+  
