code/experimental/Hacl.Spec.P384.Definition.fst
@@ -12,8 +12,42 @@ open FStar.Mul
 
 
 noextract 
-let prime384: (a: pos { a < pow2 384}) = 
+let prime384: (a: pos {a > 3 && a < pow2 384}) = 
+  assert_norm (pow2 384 - pow2 128 - pow2 96 + pow2 32 - 1 < pow2 384);
+  assert_norm (pow2 384 - pow2 128 - pow2 96 + pow2 32 - 1 > 3);
   pow2 384 - pow2 128 - pow2 96 + pow2 32 - 1
+
+
+inline_for_extraction noextract
+let p384_prime_list : x:list uint64{List.Tot.length x == 6 /\ 
+  (
+    let open FStar.Mul in 
+    let l0 = uint_v (List.Tot.index x 0) in 
+    let l1 = uint_v (List.Tot.index x 1) in 
+    let l2 = uint_v (List.Tot.index x 2) in 
+    let l3 = uint_v (List.Tot.index x 3) in 
+    let l4 = uint_v (List.Tot.index x 4) in 
+    let l5 = uint_v (List.Tot.index x 5) in 
+    l0 + l1 * pow2 64 + l2 * pow2 (2 * 64) + l3 * pow2 (3 * 64) + l4 * pow2 (4 * 64) + l5 * pow2 (5 * 64) == prime384)
+  } =
+  let open FStar.Mul in 
+  [@inline_let]
+  let x =
+    [ (u64 0x00000000ffffffff);  
+      (u64 0xffffffff00000000);
+      (u64 0xfffffffffffffffe);  
+      (u64 0xffffffffffffffff);
+      (u64 0xffffffffffffffff);
+      (u64 0xffffffffffffffff)
+    ] in
+    assert_norm(
+      0x00000000ffffffff + 
+      0xffffffff00000000 * pow2 64 + 
+      0xfffffffffffffffe * pow2 (2 * 64) +
+      0xffffffffffffffff * pow2 (3 * 64) +
+      0xffffffffffffffff * pow2 (4 * 64) +
+      0xffffffffffffffff * pow2 (5 * 64) == prime384);
+  x
 
 
 noextract
@@ -43,16 +77,16 @@ let as_nat_t_12 f =
   let (s0, s1, s2, s3, s4, s5, s6, s7, s8, s9, s10, s11) = f in
   v s0 + 
   v s1 * pow2 64 + 
-  v s2 * pow2 64 * pow2 64 +
-  v s3 * pow2 64 * pow2 64 * pow2 64 + 
-  v s4 * pow2 64 * pow2 64 * pow2 64 * pow2 64 + 
-  v s5 * pow2 64 * pow2 64 * pow2 64 * pow2 64 * pow2 64 +
-  v s6 * pow2 64 * pow2 64 * pow2 64 * pow2 64 * pow2 64 * pow2 64 +
-  v s7 * pow2 64 * pow2 64 * pow2 64 * pow2 64 * pow2 64 * pow2 64 * pow2 64 +
-  v s8 * pow2 64 * pow2 64 * pow2 64 * pow2 64 * pow2 64 * pow2 64 * pow2 64 * pow2 64 + 
-  v s9 * pow2 64 * pow2 64 * pow2 64 * pow2 64 * pow2 64 * pow2 64 * pow2 64 * pow2 64 * pow2 64 +
-  v s10* pow2 64 * pow2 64 * pow2 64 * pow2 64 * pow2 64 * pow2 64 * pow2 64 * pow2 64 * pow2 64 * pow2 64 +
-  v s11 * pow2 64 * pow2 64 * pow2 64 * pow2 64 * pow2 64 * pow2 64 * pow2 64 * pow2 64 * pow2 64 * pow2 64 * pow2 64
+  v s2 * pow2 (2 * 64) +
+  v s3 * pow2 (3 * 64) +  
+  v s4 * pow2 (4 * 64) +
+  v s5 * pow2 (5 * 64) +
+  v s6 * pow2 (6 * 64) +
+  v s7 * pow2 (7 * 64) +
+  v s8 * pow2 (8 * 64) +
+  v s9 * pow2 (9 * 64) +
+  v s10* pow2 (10 * 64) +
+  v s11 * pow2 (11 * 64)
 
 
 
@@ -66,6 +100,18 @@ let felem12_buffer = lbuffer uint64 (size 12)
 
 noextract
 let as_nat6 (h:mem) (e:felem6_buffer) : GTot nat =
+  let s = as_seq h e in
+  let s0 = s.[0] in
+  let s1 = s.[1] in
+  let s2 = s.[2] in
+  let s3 = s.[3] in
+  let s4 = s.[4] in 
+  let s5 = s.[5] in 
+  as_nat_t_6 (s0, s1, s2, s3, s4, s5)
+
+
+noextract
+let as_nat6_il (h:mem) (e:ilbuffer uint64 (size 6)) : GTot nat =
   let s = as_seq h e in
   let s0 = s.[0] in
   let s1 = s.[1] in
@@ -92,6 +138,17 @@ let as_nat12 (h: mem) (e: felem12_buffer) : GTot nat =
   let s10 = s.[10] in 
   let s11 = s.[11] in 
   as_nat_t_12 (s0, s1, s2, s3, s4, s5, s6, s7, s8, s9, s10, s11)
+
+
+noextract 
+let seq_as_nat6 (s: lseq uint64 6) : GTot nat = 
+  let s0 = s.[0] in
+  let s1 = s.[1] in
+  let s2 = s.[2] in
+  let s3 = s.[3] in
+  let s4 = s.[4] in 
+  let s5 = s.[5] in  
+  as_nat_t_6 (s0, s1, s2, s3, s4, s5)
 
 
 noextract 
