code/experimental/Hacl.Impl.P384.LowLevel.fst
@@ -1,0 +1,24 @@
+module Hacl.Impl.P384.LowLevel
+
+open FStar.HyperStack.All
+open FStar.HyperStack
+module ST = FStar.HyperStack.ST
+
+open Lib.IntTypes
+open Lib.Buffer
+
+open Hacl.Spec.P384.Definition
+
+open Hacl.Impl.LowLevel
+
+open FStar.Math.Lemmas
+
+open FStar.Mul
+open Lib.IntTypes.Intrinsics
+
+#set-options " --z3rlimit 200"
+
+inline_for_extraction
+let prime384_buffer: x: ilbuffer uint64 (size 6) {witnessed #uint64 #(size 6) x (Lib.Sequence.of_list p384_prime_list) /\ recallable x /\ seq_as_nat6 (Lib.Sequence.of_list (p384_prime_list)) == prime384} = 
+  assert_norm (seq_as_nat6 (Lib.Sequence.of_list (p384_prime_list)) == prime384);
+  createL_global p384_prime_list
